More lemmas on renaming

src/Expr.v
@@ -80,13 +80,13 @@ Inductive eval : expr -> state Z -> Z -> Prop :=
                    (VALA : [| a |] s => za)
                    (VALB : [| b |] s => zb)
                    (NZERO : ~ zb = Z.zero),
-  [| a [/] b |] s => (Z.div za zb)
+    [| a [/] b |] s => (Z.div za zb)
 
 | bs_Mod  : forall (s : state Z) (a b : expr) (za zb : Z)
                    (VALA : [| a |] s => za)
                    (VALB : [| b |] s => zb)
                    (NZERO : ~ zb = Z.zero),
-             [| a [%] b |] s => (Z.modulo za zb)
+    [| a [%] b |] s => (Z.modulo za zb)
 
 | bs_Le_T : forall (s : state Z) (a b : expr) (za zb : Z)
                    (VALA : [| a |] s => za)
@@ -98,7 +98,7 @@ Inductive eval : expr -> state Z -> Z -> Prop :=
                    (VALA : [| a |] s => za)
                    (VALB : [| b |] s => zb)
                    (OP : Z.gt za zb),
-  [| a [<=] b |] s => Z.zero
+    [| a [<=] b |] s => Z.zero
 
 | bs_Lt_T : forall (s : state Z) (a b : expr) (za zb : Z)
                    (VALA : [| a |] s => za)
@@ -128,14 +128,14 @@ Inductive eval : expr -> state Z -> Z -> Prop :=
                    (VALA : [| a |] s => za)
                    (VALB : [| b |] s => zb)
                    (OP : Z.gt za zb),
-  [| a [>] b |] s => Z.one
+    [| a [>] b |] s => Z.one
 
 | bs_Gt_F : forall (s : state Z) (a b : expr) (za zb : Z)
                    (VALA : [| a |] s => za)
                    (VALB : [| b |] s => zb)
                    (OP : Z.le za zb),
     [| a [>] b |] s => Z.zero
-
+                         
 | bs_Eq_T : forall (s : state Z) (a b : expr) (za zb : Z)
                    (VALA : [| a |] s => za)
                    (VALB : [| b |] s => zb)
@@ -165,7 +165,7 @@ Inductive eval : expr -> state Z -> Z -> Prop :=
                    (VALB : [| b |] s => zb)
                    (BOOLA : zbool za)
                    (BOOLB : zbool zb),
-  [| a [&] b |] s => (za * zb)
+    [| a [&] b |] s => (za * zb)
 
 | bs_Or   : forall (s : state Z) (a b : expr) (za zb : Z)
                    (VALA : [| a |] s => za)
@@ -276,6 +276,7 @@ Notation "C '<~' e" := (plug C e) (at level 43, no associativity).
 
 Definition contextual_equivalent (e1 e2 : expr) : Prop :=
   forall (C : Context), (C <~ e1) ~~ (C <~ e2).
+
 Notation "e1 '~c~' e2" := (contextual_equivalent e1 e2)
                             (at level 42, no associativity).
 
@@ -309,16 +310,16 @@ Module SmallStep.
                       (EVAL    : [| Bop op (Nat zl) (Nat zr) |] s => z), (s |- (Bop op (Nat zl) (Nat zr)) --> (Nat z))      
   where "st |- e --> e'" := (ss_step st e e').
 
-  Reserved Notation "st |- e => e'" (at level 0).
+  Reserved Notation "st |- e -->> e'" (at level 0).
 
   Inductive ss_eval : state Z -> expr -> expr -> Prop :=
     se_Stop : forall (s : state Z)
-                     (z : Z),  s |- (Nat z) => (Nat z)
+                     (z : Z),  s |- (Nat z) -->> (Nat z)
   | se_Step : forall (s : state Z)
                      (e e' e'' : expr)
                      (HStep : s |- e --> e')
-                     (Heval: s |- e' => e''), s |- e => e''
-  where "st |- e => e'"  := (ss_eval st e e').
+                     (Heval: s |- e' -->> e''), s |- e -->> e''
+  where "st |- e -->> e'"  := (ss_eval st e e').
   
   Definition normal_form (e : expr) : Prop :=
     forall s, ~ exists e', (s |- e --> e').   
@@ -339,12 +340,12 @@ Module SmallStep.
                          (H2   : s |- e --> e') : e' = Nat z.
   Proof. admit. Admitted.
   
-  Lemma ss_eval_stops_at_value (st : state Z) (e e': expr) (Heval: st |- e => e') : is_value e'.
+  Lemma ss_eval_stops_at_value (st : state Z) (e e': expr) (Heval: st |- e -->> e') : is_value e'.
   Proof. admit. Admitted.
   
   Lemma ss_eval_equiv (e : expr)
                       (s : state Z)
-                      (z : Z) : [| e |] s => z <-> (s |- e => (Nat z)).
+                      (z : Z) : [| e |] s => z <-> (s |- e -->> (Nat z)).
   Proof. admit. Admitted.
   
 End SmallStep.
@@ -352,10 +353,15 @@ End SmallStep.
 Module Renaming.
   
   Definition renaming := { f : id -> id | Bijective f }.
+
+  Fixpoint rename_id (r : renaming) (x : id) : id :=
+    match r with
+      exist _ f _ => f x
+    end.
   
   Fixpoint rename_expr (r : renaming) (e : expr) : expr :=
     match e with
-    | Var x => match r with exist _ f _ => Var (f x) end
+    | Var x => Var (rename_id r x) 
     | Nat n => Nat n
     | Bop op e1 e2 => Bop op (rename_expr r e1) (rename_expr r e2) 
     end.
